feat: use BitVec for FiniteKripkeFrame representation and completely characterize canonicalize function

KripkeGameAnalysis/ModalLogic/FiniteSemantics.lean
@@ -1,6 +1,7 @@
 import Init.Data.BitVec.Basic
 import Mathlib.Data.Nat.Cast.Order.Basic
 import Mathlib.Data.Fintype.Perm
+import Mathlib.Data.Finset.Max
 
 import KripkeGameAnalysis.ModalLogic.Basic
 import KripkeGameAnalysis.GenericExtras.BitVec
@@ -9,69 +10,21 @@ import KripkeGameAnalysis.GenericExtras.BitVec
 A finite Kripke frame is a Kripke frame with a finite number of vertices.
 We think of the vertices in the Kripke frame as being numbered from `0` to `frameSize - 1`, inclusive.
 
-TODO: use BitVec representation here instead and provide isomorphism + coersion to KripkeFrame instead?
+We use a `BitVec` to represent the accessibility relation of the Kripke frame.
+The `BitVec` is of size `frameSize ^ 2`, and the bit at position `i * frameSize + j` is `true`
+if there is an edge from vertex `i` to vertex `j`, and `false` otherwise.
 -/
-def FiniteKripkeFrame (frameSize : Nat) : Type := KripkeFrame (Fin frameSize)
-
-@[ext] lemma FiniteKripkeFrame.ext
-  {frameSize : Nat} {frame1 frame2 : FiniteKripkeFrame frameSize}
-  (h : ∀i j, frame1 i j = frame2 i j) : frame1 = frame2 :=
-  funext (λ i => funext (λ j => h i j))
+def FiniteKripkeFrame (frameSize : Nat) : Type := BitVec (frameSize ^ 2)
 
 namespace FiniteKripkeFrame
-  instance (frame : FiniteKripkeFrame n) : Fintype frame.vertices := inferInstanceAs (Fintype (Fin n))
-  instance (frame : FiniteKripkeFrame n) : DecidableEq frame.vertices := inferInstanceAs (DecidableEq (Fin n))
-  instance : DecidableEq (FiniteKripkeFrame n) := inferInstanceAs (DecidableEq (KripkeFrame (Fin n)))
+  def mk (n : ℕ) (v : BitVec (n ^ 2)) : FiniteKripkeFrame n := v
 
-  def allNodes (frame : FiniteKripkeFrame n) : Finset frame.vertices := Finset.univ
-  lemma allNodes_card_eq_frameSize (frame : FiniteKripkeFrame n) : frame.allNodes.card = n :=
-    by apply Fintype.card_fin
-
-  def accessibilityRelationCount (frame : FiniteKripkeFrame n) : ℕ :=
-    ((frame.allNodes.product (frame.allNodes)).filter (fun a => frame.accessible a.fst a.snd)).card
-
-  section FiniteValuation
-  structure FiniteValuation (frame : FiniteKripkeFrame n) (finVars : Type) [Fintype finVars] [DecidableEq finVars] where
-    valuation : frame.Valuation finVars
-
-  variable {finVars : Type} [Fintype finVars] [DecidableEq finVars]
-  namespace FiniteValuation
-    def equivToFinSetRepresentation {frame : FiniteKripkeFrame n}:
-                                    (frame.FiniteValuation finVars) ≃ (Finset (finVars × frame.vertices)) :=
-      let valPowersetEquiv : (frame.Valuation finVars) ≃ (Finset (finVars × frame.vertices)) := finsetProdEquivCurriedCharacteristic.symm
-      let valEquiv : (frame.FiniteValuation finVars) ≃ (frame.Valuation finVars) := {
-        toFun := fun val => val.valuation,
-        invFun := fun val => { valuation := val },
-        left_inv := by intro val; simp,
-        right_inv := by intro val; simp
-      }
-      valEquiv.trans valPowersetEquiv
-  end FiniteValuation
-
-  def allFinValuations (frame : FiniteKripkeFrame n) : Finset (frame.FiniteValuation finVars) :=
-    let valuationsAsPsets := (Finset.product (inferInstance (α := Fintype finVars)).elems frame.allNodes).powerset
-    valuationsAsPsets.map (FiniteValuation.equivToFinSetRepresentation (frame := frame).symm.toEmbedding)
-
-  def satisfiesForAllValuations {frame : FiniteKripkeFrame n} (i : frame.vertices) (fml : ModalFormula finVars) : Bool :=
-    decide (∀finval ∈ frame.allFinValuations, finval.valuation.decideSatisfaction i fml)
-
-  def countSatisfyingNodes (frame : FiniteKripkeFrame n) (fml : ModalFormula finVars) : ℕ :=
-    (frame.allNodes.filter (fun i => satisfiesForAllValuations i fml)).card
-
-  lemma countSatisfyingNodes_leq_frameSize: ∀ {frame : FiniteKripkeFrame n} {fml : ModalFormula finVars},
-                                             frame.countSatisfyingNodes fml ≤ n := by
-    intro frame fml
-    simp only [FiniteKripkeFrame.countSatisfyingNodes]
-    simp only [← frame.allNodes_card_eq_frameSize]
-    apply Finset.card_filter_le
-  end FiniteValuation
-
-  def equivSquareBoolFn : (FiniteKripkeFrame n) ≃ (Fin (n ^ 2) → Bool) :=
+  def kripkeFrameFinNEquivSquareBoolFn : KripkeFrame (Fin n) ≃ (Fin (n ^ 2) → Bool) :=
     let fin_implies_gt_zero {k : Nat} : Fin k → k > 0 := fun i => by
       have : k ≠ 0 := by intro h; rw [h] at i; exact Nat.not_lt_zero _ i.is_lt
       exact Nat.pos_of_ne_zero this
 
-    let frameToBoolFn : (FiniteKripkeFrame n) → (Fin (n ^ 2) → Bool) := fun frame i =>
+    let frameToBoolFn : KripkeFrame (Fin n) → (Fin (n ^ 2) → Bool) := fun frame i =>
       let n_gt_zero : n > 0 := by
         have n_sq_gt_zero : n ^ 2 > 0 := fin_implies_gt_zero i
         have : n ^ 2 > 0 → n > 0 := by contrapose; simp
@@ -81,7 +34,7 @@ namespace FiniteKripkeFrame
         ⟨i.val / n, by apply (Nat.div_lt_iff_lt_mul n_gt_zero).mpr; rw [←Nat.pow_two n]; exact i.is_lt⟩
         ⟨i.val % n, by exact Nat.mod_lt _ n_gt_zero⟩
 
-    let boolFnToFrame : (Fin (n ^ 2) → Bool) → (FiniteKripkeFrame n) := fun boolFn i j =>
+    let boolFnToFrame : (Fin (n ^ 2) → Bool) → KripkeFrame (Fin n) := fun boolFn i j =>
       boolFn
         ⟨i.val * n + j.val, by
           simp [Nat.pow_two]
@@ -112,40 +65,156 @@ namespace FiniteKripkeFrame
         rw [Nat.add_comm, Nat.mul_comm, Nat.mod_add_div _ _]
     }
 
-  instance : HasEquiv (FiniteKripkeFrame n) := inferInstanceAs (HasEquiv (KripkeFrame (Fin n)))
+  def equivToKripkeFrameFin: FiniteKripkeFrame n ≃ KripkeFrame (Fin n) :=
+    (BitVec.equivToBitPred (n ^ 2)).trans kripkeFrameFinNEquivSquareBoolFn.symm
+
+  instance instLinOrd : LinearOrder (FiniteKripkeFrame n) where
+    le := fun f1 f2 => (f1 : BitVec (n ^ 2)).ule f2
+    le_refl := by intro f; simp [BitVec.ule]
+    le_trans := by intro f1 f2 f3; simp [BitVec.ule]; exact Nat.le_trans
+    le_antisymm := by intro f1 f2; simp [BitVec.ule]; intro h1 h2; apply BitVec.eq_of_toNat_eq; apply Nat.le_antisymm h1 h2
+    le_total := by intro f1 f2; simp [BitVec.ule]; exact Nat.le_total _ _
+    decidableLE := fun f1 f2 => inferInstanceAs (Decidable ((f1 : BitVec (n ^ 2)).ule f2))
+  instance instCoe : Coe (FiniteKripkeFrame n) (KripkeFrame (Fin n)) where coe := equivToKripkeFrameFin.toFun
+  abbrev asKripkeFrame (frame : FiniteKripkeFrame n) : KripkeFrame (Fin n) := frame
+  instance instFunLike : FunLike (FiniteKripkeFrame n) (Fin n) (Fin n → Bool) where
+    coe frame := frame.asKripkeFrame
+    coe_injective' := by
+      intro frame1 frame2 h
+      have h' : frame1.asKripkeFrame = frame2.asKripkeFrame := h
+      simp [asKripkeFrame] at h'
+      exact h'
+  @[simp] theorem equivToKripkeFrameFin_coe (frame : FiniteKripkeFrame n) : (equivToKripkeFrameFin frame) i j = frame i j := by rfl
+
+  abbrev mkFromKripkeFrameFin (frame : KripkeFrame (Fin n)) : FiniteKripkeFrame n := equivToKripkeFrameFin.invFun frame
+  @[simp] theorem mkFromKripkeFrameFin_coe (frame : KripkeFrame (Fin n)) : (mkFromKripkeFrameFin frame) i j = frame i j := by
+    simp [mkFromKripkeFrameFin]
+    have h : DFunLike.coe (equivToKripkeFrameFin.symm frame) = frame := equivToKripkeFrameFin.right_inv frame
+    rw [h]
+  @[ext] theorem ext {frame1 frame2 : FiniteKripkeFrame n} (h : ∀i j, frame1 i j = frame2 i j) : frame1 = frame2 :=
+    instFunLike.coe_injective' (funext (λ i => funext (λ j => h i j)))
+
+  abbrev vertices (frame : FiniteKripkeFrame n) : Type := frame.asKripkeFrame.vertices
+  instance (frame : FiniteKripkeFrame n) : Fintype frame.vertices := inferInstanceAs (Fintype (Fin n))
+  instance (frame : FiniteKripkeFrame n) : DecidableEq frame.vertices := inferInstanceAs (DecidableEq (Fin n))
+
+  instance : Fintype (FiniteKripkeFrame n) := inferInstanceAs (Fintype (BitVec (n ^ 2)))
+  instance : DecidableEq (FiniteKripkeFrame n) := inferInstanceAs (DecidableEq (BitVec (n ^ 2)))
+
+  def allNodes (frame : FiniteKripkeFrame n) : Finset frame.vertices := Finset.univ
+  lemma allNodes_card_eq_frameSize (frame : FiniteKripkeFrame n) : frame.allNodes.card = n :=
+    by apply Fintype.card_fin
+
+  def accessibilityRelationCount (frame : FiniteKripkeFrame n) : ℕ :=
+    let asBitVec : BitVec (n ^ 2) := frame
+    (Finset.univ.filter (fun (i : Fin (n ^ 2)) => asBitVec[i])).card
+
+  section FiniteValuation
+  abbrev Valuation (frame : FiniteKripkeFrame n) (vars : Type) : Type := frame.asKripkeFrame.Valuation vars
+  structure FiniteValuation (frame : FiniteKripkeFrame n) (finVars : Type) [Fintype finVars] [DecidableEq finVars] where
+    valuation : frame.Valuation finVars
+
+  variable {finVars : Type} [Fintype finVars] [DecidableEq finVars]
+  namespace FiniteValuation
+    def equivToFinSetRepresentation {frame : FiniteKripkeFrame n}:
+                                    (frame.FiniteValuation finVars) ≃ (Finset (finVars × frame.vertices)) :=
+      let valPowersetEquiv : (frame.Valuation finVars) ≃ (Finset (finVars × frame.vertices)) :=
+        finsetProdEquivCurriedCharacteristic.symm
+      let valEquiv : (frame.FiniteValuation finVars) ≃ (frame.Valuation finVars) := {
+        toFun := fun val => val.valuation,
+        invFun := fun val => { valuation := val },
+        left_inv := by intro val; simp,
+        right_inv := by intro val; simp
+      }
+      valEquiv.trans valPowersetEquiv
+  end FiniteValuation
+
+  def allFinValuations (frame : FiniteKripkeFrame n) : Finset (frame.FiniteValuation finVars) :=
+    let valuationsAsPsets := (Finset.product (inferInstance (α := Fintype finVars)).elems frame.allNodes).powerset
+    valuationsAsPsets.map (FiniteValuation.equivToFinSetRepresentation (frame := frame).symm.toEmbedding)
+
+  def satisfiesForAllValuations {frame : FiniteKripkeFrame n} (i : frame.vertices) (fml : ModalFormula finVars) : Bool :=
+    decide (∀finval ∈ frame.allFinValuations, finval.valuation.decideSatisfaction i fml)
+
+  def countSatisfyingNodes (frame : FiniteKripkeFrame n) (fml : ModalFormula finVars) : ℕ :=
+    (frame.allNodes.filter (fun i => satisfiesForAllValuations i fml)).card
+
+  lemma countSatisfyingNodes_leq_frameSize: ∀ {frame : FiniteKripkeFrame n} {fml : ModalFormula finVars},
+                                             frame.countSatisfyingNodes fml ≤ n := by
+    intro frame fml
+    simp only [FiniteKripkeFrame.countSatisfyingNodes]
+    simp only [← frame.allNodes_card_eq_frameSize]
+    apply Finset.card_filter_le
+  end FiniteValuation
+
+  instance instHasEquiv : HasEquiv (FiniteKripkeFrame n) where Equiv := fun frame1 frame2 => frame1.asKripkeFrame ≈ frame2
   def UptoIso (n : Nat) := Quotient (KripkeFrame.isSetoid (Fin n))
   namespace UptoIso
     def enumerateClass(f : FiniteKripkeFrame n) : Finset (FiniteKripkeFrame n) :=
-      let permutateFrame : Equiv.Perm (Fin n) → FiniteKripkeFrame n := fun f' i j => f (f' i) (f' j)
+      let permutateFrame : Equiv.Perm (Fin n) → FiniteKripkeFrame n := fun f' =>
+        mkFromKripkeFrameFin (fun i j => f (f' i) (f' j))
       Finset.univ (α := Equiv.Perm (Fin n)).image permutateFrame
 
-    theorem enumerateClass_mem_iff (f f' : FiniteKripkeFrame n) : f' ∈ enumerateClass f ↔ f' ≈ f := by
+    theorem enumerateClass_mem_iff (f f' : FiniteKripkeFrame n) : (f' ∈ enumerateClass f) ↔ (f' ≈ f) := by
       simp [enumerateClass]
       apply Iff.intro
       · intro iso_exists
         rcases iso_exists with ⟨iso, iso_prop⟩
         simp [HasEquiv.Equiv, KripkeFrame.Isomorphic]
         exists iso
-        intro i j
-        exact (congr_fun (congr_fun iso_prop i) j).symm
+        intros i j
+        apply congrArg (· i j) at iso_prop; simp at iso_prop
+        simp [KripkeFrame.accessible]; rw [asKripkeFrame]; simp; exact iso_prop.symm
       · intro equiv
         simp [HasEquiv.Equiv, KripkeFrame.Isomorphic] at equiv
         rcases equiv with ⟨iso, iso_prop⟩
         exists iso
-        ext i j
-        exact (iso_prop i j).symm
+        ext i j; simp; exact (iso_prop i j).symm
+
+    lemma enumerateClass_self_mem (f : FiniteKripkeFrame n) : f ∈ enumerateClass f := by
+      apply (enumerateClass_mem_iff f f).mpr
+      exact (KripkeFrame.isomorphism_equivalence.refl _)
+
+    theorem enumerateClass_equiv_eq (f f' : FiniteKripkeFrame n) : enumerateClass f = enumerateClass f' ↔ f ≈ f' := by
+      apply Iff.intro
+      · intro h
+        have f_mem_enumerateClass_f' : f ∈ enumerateClass f' := by rw [←h]; exact enumerateClass_self_mem f
+        exact (enumerateClass_mem_iff f' f).mp f_mem_enumerateClass_f'
+      · intro h
+        ext a
+        apply Iff.intro
+        · intro h'
+          apply (enumerateClass_mem_iff _ _).mpr
+          apply (enumerateClass_mem_iff _ _).mp at h'
+          exact (KripkeFrame.isomorphism_equivalence.trans h' h)
+        · intro h'
+          apply (enumerateClass_mem_iff _ _).mpr
+          apply (enumerateClass_mem_iff _ _).mp at h'
+          exact (KripkeFrame.isomorphism_equivalence.trans h' (KripkeFrame.isomorphism_equivalence.symm h))
+
+    def canonicalize (f : FiniteKripkeFrame n) : FiniteKripkeFrame n :=
+      let classOf_f := enumerateClass f
+      let nonempty : classOf_f.Nonempty := by have : f ∈ classOf_f := enumerateClass_self_mem f; exists f
+      classOf_f.min' nonempty
+
+    theorem canonicalize_equiv_self (f : FiniteKripkeFrame n) : (canonicalize f) ≈ f := by
+      simp [canonicalize]
+      set lhs := (enumerateClass f).min' _
+      have lhs_in_class_f : lhs ∈ enumerateClass f := Finset.min'_mem _ _
+      exact (enumerateClass_mem_iff f lhs).mp lhs_in_class_f
+
+    theorem canonicalize_eq_iff_equiv (f f' : FiniteKripkeFrame n) : canonicalize f = canonicalize f' ↔ f ≈ f' := by
+      apply Iff.intro
+      · intro h
+        have p1 : f ≈ canonicalize f := KripkeFrame.isomorphism_equivalence.symm (canonicalize_equiv_self f)
+        rw [h] at p1
+        exact (KripkeFrame.isomorphism_equivalence.trans p1 (canonicalize_equiv_self f'))
+      · intro h
+        simp [canonicalize]
+        have enumerateClass_f_eq := (enumerateClass_equiv_eq f f').mpr h
+        simp [enumerateClass_f_eq]
+
+    theorem canonicalize_weakly_regressive : canonicalize f ≤ f := by
+      simp [canonicalize]; apply Finset.min'_le _ _; exact enumerateClass_self_mem f
   end UptoIso
-end FiniteKripkeFrame
-
-def FiniteKripkeFrameBitVecRepr (frameSize : Nat) : Type := BitVec (frameSize ^ 2)
-namespace FiniteKripkeFrameBitVecRepr
-  def equiv: (FiniteKripkeFrame n) ≃ (FiniteKripkeFrameBitVecRepr n) :=
-    FiniteKripkeFrame.equivSquareBoolFn.trans (BitVec.equivToBitPred (n ^ 2)).symm
-
-  instance : Fintype (FiniteKripkeFrameBitVecRepr n) := inferInstanceAs (Fintype (BitVec (n ^ 2)))
-end FiniteKripkeFrameBitVecRepr
-
-namespace FiniteKripkeFrame
-  instance : Fintype (FiniteKripkeFrame n) :=
-    Fintype.ofEquiv (FiniteKripkeFrameBitVecRepr n) FiniteKripkeFrameBitVecRepr.equiv.symm
 end FiniteKripkeFrame
